Add a #conflicts metric in benchmark mode

app/conflict_counter.ml
@@ -1,0 +1,5 @@
+let value = ref 0
+
+let increment () = incr value
+let reset () = value := 0
+let get () = !value
