app/conflict_counter.mli
@@ -1,0 +1,3 @@
+val increment : unit -> unit
+val reset : unit -> unit
+val get : unit -> int
